Fix project/confine scoping

Compiler/ProtectConfine.v
@@ -1,36 +1,53 @@
-Require Stlc.SpecSyntax.
-Require Stlc.SpecEvaluation.
-Require Stlc.SpecTyping.
-Require Stlc.LemmasTyping.
+Require Import Db.Lemmas.
 Require Import Utlc.SpecSyntax.
 Require Import Utlc.SpecEvaluation.
 Require Import Utlc.LemmasScoping.
 Require Import LogRel.PseudoType.
+Require Import LogRel.LemmasPseudoType.
 Require Import LogRel.LR.
 Require Import Erase.
+Require Import Common.Relations.
 
 Fixpoint protect (ty : S.Ty) : U.UTm :=
   abs (match ty with
          | S.tunit => var 0
          | S.tbool => var 0
-         | S.tarr ty1 ty2 => abs (app (protect ty2) (app (var 1) (app (confine ty1) (var 0))))
-         | S.tprod ty1 ty2 => pair (app (protect ty1) (proj₁ (var 0))) (app (protect ty2) (proj₂ (var 0)))
-         | S.tsum ty1 ty2 => caseof (var 0) (inl (app (protect ty1) (var 0))) (inr (app (protect ty2) (var 0)))
+         | S.tarr ty1 ty2 => abs (app (protect ty2)[wkms 2] (app (var 1) (app (confine ty1)[wkms 2] (var 0))))
+         | S.tprod ty1 ty2 => pair (app (protect ty1)[wkm] (proj₁ (var 0))) (app (protect ty2)[wkm] (proj₂ (var 0)))
+         | S.tsum ty1 ty2 => caseof (var 0) (inl (app (protect ty1)[wkms 2] (var 0))) (inr (app (protect ty2)[wkms 2] (var 0)))
        end)
 with confine (ty : S.Ty) : U.UTm :=
   abs (match ty with
          | S.tunit => seq (var 0) unit
          | S.tbool => ite (var 0) true false
-         | S.tarr ty1 ty2 => abs (app (confine ty2) (app (var 1) (app (protect ty1) (var 0))))
-         | S.tprod ty1 ty2 => pair (app (confine ty1) (proj₁ (var 0))) (app (confine ty2) (proj₂ (var 0)))
-         | S.tsum ty1 ty2 => caseof (var 0) (inl (app (confine ty1) (var 0))) (inr (app (confine ty2) (var 0)))
+         | S.tarr ty1 ty2 => abs (app (confine ty2)[wkms 2] (app (var 1) (app (protect ty1)[wkms 2] (var 0))))
+         | S.tprod ty1 ty2 => pair (app (confine ty1)[wkm] (proj₁ (var 0))) (app (confine ty2)[wkm] (proj₂ (var 0)))
+         | S.tsum ty1 ty2 => caseof (var 0) (inl (app (confine ty1)[wkms 2] (var 0))) (inr (app (confine ty2)[wkms 2] (var 0)))
        end).
 
+Lemma protect_wkm_beta1 {τ tu} :
+  (protect τ)[wkm][beta1 tu] = protect τ.
+Proof. apply apply_wkm_beta1_cancel. Qed.
+
+Lemma protect_wkm2_beta1 {τ tu} :
+  (protect τ)[wkms 2][(beta1 tu)↑] = (protect τ)[wkm].
+Proof. rewrite ap_comp; reflexivity. Qed.
+
+Lemma confine_wkm_beta1 {τ tu} :
+  (confine τ)[wkm][beta1 tu] = confine τ.
+Proof. apply apply_wkm_beta1_cancel. Qed.
+
+Lemma confine_wkm2_beta1 {τ tu} :
+  (confine τ)[wkms 2][(beta1 tu)↑] = (confine τ)[wkm].
+Proof. rewrite ap_comp; reflexivity. Qed.
 
 Local Ltac crush :=
-  repeat (try intros;
-          simpl;
-          intuition; 
+  repeat (cbn in *;
+          subst*;
+          repeat rewrite
+            ?protect_wkm_beta1, ?protect_wkm2_beta1,
+            ?confine_wkm_beta1, ?confine_wkm2_beta1,
+            ?apply_up_def_O, ?apply_up_def_S;
           repeat crushUtlcScoping;
           repeat crushUtlcSyntaxMatchH;
           repeat crushUtlcEvaluationMatchH;
@@ -40,38 +57,124 @@ Local Ltac crush :=
                    | [ H: OfType _ _ _  |- _ ] => destruct H as [[? ?] ?]
                    | [ H: OfTypeStlc _ _  |- _ ] => destruct H as [? ?]
                  end;
-          S.crushTyping
+          S.crushTyping;
+          trivial
          ).
-  
-Lemma protect_confine_closed {τ} :
-  ⟨ 0 ⊢ protect τ ⟩ ∧ 
-  ⟨ 0 ⊢ confine τ ⟩.
+
+(* These should probably be made globally opaque
+   in the Db library.
+ *)
+Local Opaque wkms.
+Local Opaque up.
+
+Lemma protect_closed {τ} : ⟨ 0 ⊢ protect τ ⟩
+with confine_closed {τ}: ⟨ 0 ⊢ confine τ ⟩.
 Proof.
-  induction τ; simpl; crush.
-  (* weakening for well-scopedness *)
-Admitted.
-  
+  - induction τ; crush;
+    try apply weakening; auto;
+    try apply (weakenings 2); auto.
+  - induction τ; crush;
+    try apply weakening; auto;
+    try apply (weakenings 2); auto.
+Qed.
+
 Lemma protect_confine_terminate {τ vu} :
   OfTypeUtlc (embed τ) vu →
-  exists vu', U.Value vu' ∧ 
-              forall Cu, U.ECtx Cu → 
-                         (U.pctx_app (U.app (protect τ) vu) Cu) -->* (U.pctx_app vu' Cu).
+  ∃ vu', U.Value vu' ∧
+    ∀ Cu, U.ECtx Cu →
+          (U.pctx_app (U.app (protect τ) vu) Cu) -->* (U.pctx_app vu' Cu).
 Proof.
   revert vu.
   induction τ; crush.
   - (* ptarr τ₁ τ₂ *)
-    exists (abs (app (protect τ2) (app vu (app (confine τ1) (var 0))))).
-    crush. 
-    enough (U.pctx_app
-              (U.app
-                 (abs (abs (app (protect τ2) (app (var 1) (app (confine τ1) (var 0))))))
-                 vu) Cu -->
-              U.pctx_app (abs (app (protect τ2) (app vu (app (confine τ1) (var 0))))) Cu) by eauto with eval.
-    refine (U.eval_ctx₀ _ _ _); crush.
-    replace (abs (app (protect τ2) (app vu (app (confine τ1) (var 0))))) with ((abs (app (protect τ2) (app (var 1) (app (confine τ1) (var 0))))) [beta1 vu]).
-    + refine (U.eval_beta _); crush.
-      destruct vu; crush.
-    + simpl. repeat f_equal.
-      (* Problem: no assumption currently that OfType values are closed *) 
-      (* Problem: closedness implies that substitution has no effect: lemma missing? *) 
+    destruct vu; crush.
+    exists
+      (abs
+         (app
+            (protect τ2)[wkm]
+            (app
+               (abs vu[wkm↑])
+               (app (confine τ1)[wkm] (var 0))))).
+    crush.
+    apply evalToStar, U.eval_ctx₀; crush.
+    apply U.eval_beta''; crush.
+  - (* ptunit *)
+    exists U.unit.
+    crush.
+    apply evalToStar, U.eval_ctx₀; crush.
+    apply U.eval_beta''; crush.
+  - (* ptbool *)
+    assert (Value vu) by (destruct H; subst; crush).
+    exists vu.
+    crush.
+    apply evalToStar, U.eval_ctx₀; crush.
+    apply U.eval_beta''; crush.
+  - (* ptprod *)
+    destruct vu; try contradiction.
+    destruct H as [ot1 ot2].
+    specialize (IHτ1 vu1 ot1); destruct IHτ1 as (vu1' & vvu1' & hyp1).
+    specialize (IHτ2 vu2 ot2); destruct IHτ2 as (vu2' & vvu2' & hyp2).
+    exists (U.pair vu1' vu2'); crush.
+    apply (evalStepStar
+             (U.pctx_app
+               (pair (app (protect τ1) (proj₁ (U.pair vu1 vu2)))
+                  (app (protect τ2) (proj₂ (U.pair vu1 vu2))))
+               Cu)).
+    apply U.eval_ctx₀; crush.
+    eapply U.eval_beta''; crush;
+      eauto using OfTypeUtlc_implies_Value.
+    apply (evalStepStar
+             (U.pctx_app
+                (pair (app (protect τ1) vu1)
+                   (app (protect τ2) (proj₂ (U.pair vu1 vu2)))) Cu)).
+    admit.
+    apply (evalStepStar
+             (U.pctx_app
+                (pair vu1'
+                   (app (protect τ2) (proj₂ (U.pair vu1 vu2)))) Cu)).
+    admit.
+    apply (evalStepStar
+             (U.pctx_app
+                (pair vu1'
+                   (app (protect τ2) vu2)) Cu)).
+    admit.
+    admit.
+  - (* ptsum *)
+    destruct vu; try contradiction;
+      [ rename IHτ1 into IH | rename IHτ2 into IH ];
+      specialize (IH vu H); destruct IH as (vu' & vvu' & hyp);
+      assert (vvu: Value vu) by eauto using OfTypeUtlc_implies_Value;
+      exists vu'; crush.
+    + apply (evalStepStar
+               (U.pctx_app
+                  (caseof
+                     (U.inl vu)
+                     (inl (app (protect τ1)[wkm] (var 0)))
+                     (inr (app (protect τ2)[wkm] (var 0))))
+                  Cu)).
+      apply U.eval_ctx₀; crush.
+      apply U.eval_beta''; crush.
+      apply (evalStepStar
+               (U.pctx_app
+                 (inl (app (protect τ1) vu))
+                 Cu)).
+      apply U.eval_ctx₀; crush.
+      eapply eval₀_case_inl'; crush.
+      admit.
+    + apply (evalStepStar
+               (U.pctx_app
+                  (caseof
+                     (U.inr vu)
+                     (inl (app (protect τ1)[wkm] (var 0)))
+                     (inr (app (protect τ2)[wkm] (var 0))))
+                  Cu)).
+      apply U.eval_ctx₀; crush.
+      apply U.eval_beta''; crush.
+      apply (evalStepStar
+               (U.pctx_app
+                 (inr (app (protect τ2) vu))
+                 Cu)).
+      apply U.eval_ctx₀; crush.
+      eapply eval₀_case_inr'; crush.
+      admit.
 Admitted.
